src/polytime.lean
@@ -37,3 +37,37 @@ by { induction v, { exact polytime_nil, }, apply polytime_node; assumption }
 lemma polytime_ite {c₁ c₂ c₃ : code} (p₁ : polytime c₁) (p₂ : polytime c₂) (p₃ : polytime c₃) :
   polytime (code.ite c₁ c₂ c₃) :=
 polytime_comp (polytime_case p₂ p₃) (polytime_node p₁ polytime_id)
+
+lemma polytime_ite' {c₁ c₂ c₃ : code} (p₁ : polytime c₁) (p₂ p₃ : polynomial ℕ)
+  (hp₂ : ∀ (n : ℕ) (x : ptree), x.sizeof ≤ n → ptree.nil ∈ c₁.eval x → ∃ t ∈ c₂.time x, t ≤ p₂.eval n)
+  (hp₃ : ∀ (n : ℕ) (x : ptree), x.sizeof ≤ n → ptree.nil ∉ c₁.eval x → ∃ t ∈ c₃.time x, t ≤ p₃.eval n) :
+  polytime (c₁.ite c₂ c₃) :=
+begin
+  have ite_dom_univ : (c₁.ite c₂ c₃).eval.dom = set.univ,
+  { rw dom_univ_iff, intro x, rw ite_dom,
+    obtain ⟨r, hr⟩ := part.dom_iff_mem.mp (p₁.dom_univ' x), use [r, hr],
+    split,
+    { rintro rfl, rw [← time_dom_iff_eval_dom, part.dom_iff_mem],
+      obtain ⟨y, hy, _⟩ := hp₂ _ _ rfl.le hr, exact ⟨y, hy⟩, },
+    { intro h, rw [← time_dom_iff_eval_dom, part.dom_iff_mem],
+      obtain ⟨y, hy, _⟩ := hp₃ _ x rfl.le (λ C, h (part.mem_unique hr C)), exact ⟨y, hy⟩, } },
+  have cond_dom_univ : ∀ x, (c₁.eval x).dom := p₁.dom_univ',
+  rcases p₁ with ⟨p₁, e₁⟩,
+  use p₁ + p₂ + p₃ + (polynomial.monomial 1 1) + 3,
+  intros n v hnv,
+  rw [← time_dom_eq_eval_dom, dom_univ_iff] at ite_dom_univ, specialize ite_dom_univ v,
+  rw part.dom_iff_mem at ite_dom_univ, cases ite_dom_univ with t H, use [t, H],
+  specialize cond_dom_univ v, specialize e₁ n v hnv, specialize hp₂ n v hnv, specialize hp₃ n v hnv,
+  obtain ⟨r, hr⟩ := part.dom_iff_mem.mp cond_dom_univ,
+  obtain ⟨tc, htc, tc_le⟩ := e₁,
+  rw ← part.eq_some_iff at hr htc,
+  simp [code.ite, code.time, hr, htc, add_def] at H,
+  rcases H with ⟨t, ht, rfl⟩,
+  suffices : t ≤ p₂.eval n + p₃.eval n,
+  { simp at ⊢, linarith only [this, tc_le, hnv], },
+  split_ifs at ht,
+  { subst h, simp [hr] at hp₂, rcases hp₂ with ⟨t, ht', Ht⟩, cases part.mem_unique ht ht',
+    nlinarith only [Ht], },
+  { rw (@comm _ (=)) at h, simp [hr, h] at hp₃, rcases hp₃ with ⟨t, ht', Ht⟩, cases part.mem_unique ht ht',
+    nlinarith only [Ht], },
+end
